new

BB_generation.v
@@ -11,10 +11,6 @@ Require Export Bool.
 Require Export Lia.
 
 
-
-(* Create a global variable recording the current block number *)
-Definition global_block_num : nat := 0.
-  
 Inductive JumpKind : Type :=
 | UJump  (* Represents an unconditional jump *)
 | CJump.   (* Represents a conditional jump *)
@@ -32,13 +28,14 @@ Record BlockInfo : Type := {
 (* Definition of BasicBlock *)
 Record BasicBlock : Type := {
   block_num : nat; (* Represents the block's identifier *)
-  commands : list cmd; (* Represents a command *)
+  commands : list BB_cmd; (* Represents a command *)
   jump_info : BlockInfo (* Defines the jump information *)
 }.
 
+
 Notation "s '.(block_num)'" := (block_num s) (at level 1).
 Notation "s '.(cmd)'" := (commands s) (at level 1).
-Notation "s '.(jmp)'" := (jump_info s) (at level 1).
+Notation "s '.(jump_info)'" := (jump_info s) (at level 1).
 
 
 (* Definition
@@ -48,211 +45,207 @@ Notation "s '.(jmp)'" := (jump_info s) (at level 1).
 *)
 
 Record basic_block_gen_results : Type := {
-  BasicBlocks: list BasicBlock;
-  current_block_num: nat
+  BasicBlocks: list BasicBlock; (* already finished blocks*)
+  BBn: BasicBlock; (* current_block_num should be the block num of BB_now, I think *)
+  next_block_num: nat (* I think next block should start with the number*)
 }.
 
-(* Definition of the length of a command *)
+Notation "s '.(BasicBlocks)'" := (BasicBlocks s) (at level 1).
+Notation "s '.(next_block_num)'" := (next_block_num s) (at level 1).
+Notation "s '.(BBn)'"  := (BBn s)(at level 1).
+
+(* 空基本块，用于寻找BB list中最后一个元素时候的默认值处理*)
+Definition EmptyBlock : BasicBlock := {|
+  block_num := 10;
+  commands := [];
+  jump_info := {|
+    jump_kind := UJump;
+    jump_dist_1 := 9; (* default endinfo *)
+    jump_dist_2 := None;
+    jump_condition := None
+  |}
+|}.
+
+(*名字瞎起的，可以改一下*)
+(*When finishing all block generations,
+the record still remains a BBs and a BBn, which is indeed completed.
+This function merge the result to a whole list of basicblock*)
+Definition to_result (r: basic_block_gen_results) :
+list BasicBlock := r.(BasicBlocks) ++ [r.(BBn)].
 
 
-Program Fixpoint basic_block_gen (cmds: list cmd) (BB_now: BasicBlock) {measure (cmd_list_len cmd_len cmds)}: basic_block_gen_results:=
+(*考虑将已经生成的所有basicblock作为输入*)
+Section basic_block_gen.
+
+Variable cmd_BB_gen : cmd -> list BasicBlock -> BasicBlock -> nat -> basic_block_gen_results.
+
+(*Parameters:
+  cmds: list of commands that need to be managed
+  BBs: list of Basic Blocks which have been already generated
+  BB_now: the Basic Block we are currently at
+  BB_num: we should start assigning new basic blocks with BB_num *)
+Fixpoint list_cmd_BB_gen (cmds: list cmd) (BBs: list BasicBlock)(BB_now: BasicBlock)(BB_num: nat): basic_block_gen_results :=
   match cmds with
-  | [] =>
-    (* No more commands, return the current basic block *)
-    {| BasicBlocks := [BB_now]; current_block_num := BB_now.(block_num) |}
- 
-    (* 这里是表示取列表的头元素为CAsgn的情况，:: tl表示的是[列表剩下的所有元素] *)
-  | CAsgn x e :: tl =>
-    (* Add the assignment command to the current basic block *)
-    let BB_next := {|
-      block_num := BB_now.(block_num); (* 这里block_num是不改的 *)
-      commands := BB_now.(commands) ++ [CAsgn x e]; (* 这里是把CAsgn x e加到commands的末尾 *)
-      jump_info := BB_now.(jump_info) (* 这里其实还是空 *)
-    |} in
-    basic_block_gen tl BB_next (* 用剩下的cmd和更新后的BB来进一步递归 *)
-
-  | CIf e c1 c2 :: tl =>
-    (*
-        Structure: If | Then | Else | Next, each of them represents a basic block
-        Corresponds to BB_now' | BB_then | BB_else | BB_next
-        Block_num is set to be a | a + 2 ~ b | b + 1 ~ c | a + 1
-    *)
-    let BB_next := {|
-      block_num := S(BB_now.(block_num)); (* a + 1 *)
-      commands := []; (* 创建一个空的命令列表 *)
-      (* 占位符，后续在递归中会修改 *)
-      jump_info := {|
-        jump_kind := UJump;
-        jump_dist_1 := 0;
-        jump_dist_2 := None;
-        jump_condition := None
-      |}
-    |} in
-
-    let BB_then := {|
-      block_num := S (BB_next.(block_num)); (* a + 2 *)
-      commands := c1;
-      jump_info := {|
-        jump_kind := UJump;
-        jump_dist_1 := BB_next.(block_num); 
-        jump_dist_2 := None; 
-        jump_condition := None
-      |}
-    |} in
-
-    let BB_then_generated_results := basic_block_gen c1 BB_then in
-
-    let BB_else := {|
-      block_num := S (BB_then_generated_results.(current_block_num)); (* current block num +1 *)
-      commands := c2;
-      jump_info := {|
-        jump_kind := UJump;
-        jump_dist_1 := BB_next.(block_num); (* a + 1 *)
-        jump_dist_2 := None; 
-        jump_condition := None
-      |}
-    |} in
-
-    let BB_else_generated_results := basic_block_gen c2 BB_else in
-
-    let BB_now' := {|
-      block_num := BB_now.(block_num);
-      commands := BB_now.(commands);
-      jump_info := {|
-        jump_kind := CJump;
-        jump_dist_1 := BB_then.(block_num);
-        jump_dist_2 := Some (BB_else.(block_num));
-        jump_condition := Some (e);
-      |}
-    |} in
-
-    let BB_next_generated_results := basic_block_gen tl BB_next in
-    {| BasicBlocks := [BB_now'] ++ BB_then_generated_results.(BasicBlocks) ++ BB_else_generated_results.(BasicBlocks) ++ BB_next_generated_results.(BasicBlocks);
-       current_block_num := BB_else_generated_results.(current_block_num) |}
-  | CWhile pre e body :: tl => 
-      (*
-          Structure: Now | Pre | Body | Next, each of them represents a basic block
-          Corresponds to BB_now' | BB_pre | BB_else | BB_next
-          Block_num is set to be a | a + 2 ~ b | b + 1 ~ c| a + 1
-      *)
-    
-    let BB_next := {|
-      block_num := S(BB_now.(block_num)); (* a + 1 *)
-      commands := []; (* 创建一个空的命令列表 *)
-      (* 占位符，后续在递归中会修改 *)
-      jump_info := {|
-        jump_kind := UJump;
-        jump_dist_1 := 0;
-        jump_dist_2 := None;
-        jump_condition := None
-      |}
-    |} in
-    
-    (* 占位，因为pre中要知道自己需要产生多少个BB，来指定自己跳转的位置 (到Body) *)
-    let BB_pre' := {|
-      block_num := S (BB_next.(block_num)); (* a + 2 *)
-      commands := pre;
-      jump_info := {|
-        jump_kind := CJump;
-        jump_dist_1 := S (S (BB_next.(block_num))); (* a + 3 *)
-        jump_dist_2 := Some BB_next.(block_num); (* jump out of the loop *)
-        jump_condition := Some e
-      |}
-    |} in
-
-    let BB_pre_generated_results := basic_block_gen pre BB_pre' in
-
-    let BB_pre := {|
-      block_num := S (BB_next.(block_num)); (* a + 2 *)
-      commands := pre;
-      jump_info := {|
-        jump_kind := CJump;
-        jump_dist_1 := S (S (BB_next.(block_num))); (* a + 3 *)
-        jump_dist_2 := Some BB_next.(block_num); (* jump out of the loop *)
-        jump_condition := Some e
-      |}
-    |} in
-
-    let BB_body := {|
-      block_num := S (BB_pre_generated_results.(current_block_num)); (* b + 1 *)
-      commands := body;
-      jump_info := {|
-        jump_kind := UJump;
-        jump_dist_1 := BB_pre.(block_num); (* a + 2 *)
-        jump_dist_2 := None;
-        jump_condition := None
-      |}
-    |} in
-
-    let BB_body_generated_results := basic_block_gen body BB_body in
-
-    let BB_now' := {|
-      block_num := BB_now.(block_num);
-      commands := BB_now.(commands);
-      jump_info := {|
-        jump_kind := UJump;
-        jump_dist_1 := BB_pre.(block_num);
-        jump_dist_2 := None;
-        jump_condition := None
-      |}
-    |} in
-
-    let BB_next_generated_results := basic_block_gen tl BB_next in
-
-    {| BasicBlocks := [BB_now'] ++ BB_pre_generated_results.(BasicBlocks) ++ BB_body_generated_results.(BasicBlocks) ++ BB_next_generated_results.(BasicBlocks);
-      current_block_num := BB_body_generated_results.(current_block_num) |}
+  | [] => {| BasicBlocks := BBs; BBn := BB_now; next_block_num := BB_num;  |}
+  | cmd :: tl => 
+    let cmd_BB_result := cmd_BB_gen (cmd) (BBs) (BB_now) (BB_num) in  (* 先对列表第一个cmd进行处理，返回results *)
+    let tl_BB_result := list_cmd_BB_gen (tl) (cmd_BB_result.(BasicBlocks))(cmd_BB_result.(BBn)) (cmd_BB_result.(next_block_num)) in  (* 对剩下的cmd进行处理，返回results *)
+    tl_BB_result
   end.
 
-Next Obligation.
-Proof.
-  intros.
-  induction c2 as [| c2_head c2_tail]; simpl.
-  - lia.
-  - lia.
-Qed.
-Next Obligation.
-Proof.
-  intros.
-  induction c1 as [| c1_head c1_tail]; simpl.
-  - lia.
-  - lia.
-Qed.
-Next Obligation.
-Proof.
-  intros.
-  induction tl as [| tl_head tl_tail]; simpl.
-  - lia.
-  - lia.
-Qed.
-(* IF Proof Completed *)
-Next Obligation.
-Proof.
-  intros.
-  induction pre as [| pre_head pre_tail]; simpl.
-  - lia.
-  - lia. 
-Qed.
-Next Obligation.
-Proof.
-  intros.
-  induction body as [| body_head body_tail]; simpl.
-  - lia.
-  - lia.
-Qed.
 
-Next Obligation.
-Proof.
-  intros.
-  induction tl as [| tl_head tl_tail]; simpl.
-  - lia.
-  - lia.
-Qed.
+  
+End basic_block_gen.
 
 
-Definition get_basic_block_gen_num (cmds: list cmd) (BB_now: BasicBlock) : nat :=
-  (basic_block_gen cmds BB_now).(current_block_num).
+(*Parameters:
+  c: the cmd we are currently facing
+  BBs: list of Basic Blocks which have been already generated
+  BB_now: the Basic Block we are currently at
+  BB_num: we should start assigning new basic blocks with BB_num *)
+Fixpoint cmd_BB_gen (c: cmd) (BBs: list BasicBlock)(BB_now: BasicBlock) (BB_num: nat) : basic_block_gen_results :=
+  match c with
+  | CAsgn x e => 
+    (* update BB_now *)
+    let BB_cmd := {|
+      X := x;
+      E := e
+    |} in
+
+    let BB_now' := {|
+      block_num := BB_now.(block_num);
+      commands := BB_now.(commands) ++ [BB_cmd];
+      jump_info := BB_now.(jump_info)
+    |} in
+    {| 
+      BasicBlocks := BBs;
+      BBn := BB_now';
+      next_block_num := BB_num
+    |}
+
+  | CIf e c1 c2 =>
+    let BB_then_num := BB_num in
+    let BB_else_num := S(BB_then_num) in
+    let BB_next_num := S(BB_else_num) in
+    let BB_num1 := S(BB_next_num) in
+    let BB_now' := {|
+      block_num := BB_now.(block_num);
+      commands := BB_now.(commands);
+      jump_info := {|
+        jump_kind := CJump;
+        jump_dist_1 := BB_then_num;
+        jump_dist_2 := Some (BB_else_num);
+        jump_condition := Some (e);
+        |}
+      |} in
+
+    let BB_then := {|
+      block_num := BB_then_num;
+      commands := [];
+      jump_info := {|
+        jump_kind := UJump;
+        jump_dist_1 := BB_next_num; 
+        jump_dist_2 := None; 
+        jump_condition := None
+      |}
+    |} in
+
+    let BB_then_generated_results := list_cmd_BB_gen cmd_BB_gen c1 (BBs++[BB_now']) BB_then BB_num1 in
+
+    let BB_num2 := BB_then_generated_results.(next_block_num) in
+
+    let BB_else := {|
+      block_num := BB_else_num;
+      commands := [];
+      jump_info := {|
+        jump_kind := UJump;
+        jump_dist_1 := BB_next_num; 
+        jump_dist_2 := None; 
+        jump_condition := None
+      |}
+    |} in
+
+    let BB_else_generated_results := list_cmd_BB_gen cmd_BB_gen c2 (to_result(BB_then_generated_results)) BB_else BB_num2 in
+  
+    let BB_num3 := BB_else_generated_results.(next_block_num) in
+
+    let BB_next := {|
+      block_num := BB_next_num;
+      commands := []; (* 创建一个空的命令列表 *)
+      jump_info := BB_now.(jump_info)
+      |} in
+
+    {| BasicBlocks := to_result(BB_else_generated_results);
+       BBn := BB_next;
+       next_block_num := BB_num3 |}
+    
+  | CWhile pre e body => 
+
+    let BB_pre_num := BB_num in 
+    let BB_body_num := S(BB_pre_num) in 
+    let BB_next_num := S (BB_body_num) in
+    let BB_num1 := S(BB_next_num) in
+
+    let BB_now' := {|
+      block_num := BB_now.(block_num); 
+      commands := BB_now.(commands);
+      jump_info := {|
+        jump_kind := UJump;
+        jump_dist_1 := BB_pre_num; (* update jump info*)
+        jump_dist_2 := None;
+        jump_condition := None
+      |}
+    |} in
+
+    let BB_pre := {|
+    block_num := BB_pre_num; 
+    commands := [];
+    jump_info := {|
+      jump_kind := CJump;
+      jump_dist_1 := BB_body_num; (* jump to the body *)
+      jump_dist_2 := Some BB_next_num; (* jump out of the loop *)
+      jump_condition := Some e
+      |}
+    |} in
+    
+    let BB_pre_generated_results := list_cmd_BB_gen cmd_BB_gen pre (BBs++[BB_now']) BB_pre BB_num1 in
+
+    let BB_num2 := BB_pre_generated_results.(next_block_num) in
+
+    let BB_body := {|
+      block_num := BB_body_num;
+      commands := [];
+      jump_info := {|
+        jump_kind := UJump;
+        jump_dist_1 := BB_pre_num; 
+        jump_dist_2 := None;
+        jump_condition := None
+      |}
+    |} in
+
+    let BB_body_generated_results := list_cmd_BB_gen cmd_BB_gen body (to_result(BB_pre_generated_results)) BB_body BB_num2 in
+    
+    let BB_num3 := BB_body_generated_results.(next_block_num) in
+
+    let BB_next := {|
+      block_num := BB_next_num;
+      commands := [];
+      jump_info := BB_now.(jump_info)
+    |} in
+      
+    {| BasicBlocks := to_result(BB_pre_generated_results) ; 
+      BBn := BB_next;
+       next_block_num := BB_num3 |}
+  end.
 
 
-Definition get_basic_block_gen_list (cmds: list cmd) (BB_now: BasicBlock) : list BasicBlock :=
-  (basic_block_gen cmds BB_now).(BasicBlocks).
+Check cmd_BB_gen.
+
+
+(* main function, which generates BBs for the whole cmds. Take zero as start for now*)
+Definition BB_gen (cmds: list cmd):
+list BasicBlock := to_result (list_cmd_BB_gen cmd_BB_gen cmds [] EmptyBlock 11).
+
+
+
 
