BB_denotations.v
@@ -1,0 +1,380 @@
+Require Import Coq.micromega.Psatz.
+Require Import Coq.ZArith.ZArith.
+Require Import Coq.Strings.String.
+Require Import Coq.Classes.Morphisms.
+Require Import SetsClass.SetsClass. 
+Import SetsNotation.
+Require Import compcert.lib.Integers.
+Local Open Scope bool.
+Local Open Scope string.
+Local Open Scope Z.
+Local Open Scope sets.
+Require Import Main.grammer.
+Require Import Main.cmd_denotations.
+Require Import Main.BB_generation.
+Require Import Coq.Lists.List.
+Import Denotation.
+Import EDenote.
+Import CDenote.
+Import EmptyEDenote.
+
+Record BB_state: Type := {
+  BB_num: nat;
+  st: state
+}.
+
+Module BDenote.
+Record BDenote: Type := {
+  Bnrm: BB_state -> BB_state -> Prop;
+  Berr: BB_state -> Prop;
+  Binf: BB_state -> Prop
+}.
+End BDenote.
+
+Import BDenote.
+
+Definition empty_sem : BDenote := {|
+  Bnrm := ∅;
+  Berr := ∅;
+  Binf := ∅
+|}.
+
+Definition get_state (bs: BB_state): state := bs.(st).
+
+
+
+Definition test_true_jmp (D: EDenote):
+  state -> Prop :=
+    (fun s => exists i, D.(nrm) s i /\ Int64.signed i <> 0).
+
+Definition test_false_jmp (D: EDenote):
+  state -> Prop :=
+    (fun s => D.(nrm) s (Int64.repr 0)).
+
+Definition ujmp_sem (jum_dist: nat): BDenote :=
+  {|
+    Bnrm := fun (bs1: BB_state) (bs2 :BB_state) =>
+      bs1.(st) = bs2.(st) /\ bs2.(BB_num) = jum_dist;
+    Berr := ∅;
+    Binf := ∅;
+  |}.
+
+Definition cjmp_sem (jmp_dist1: nat) (jmp_dist2: nat) (D: EDenote) : BDenote :=
+  {|
+    Bnrm := fun bs1 bs2 => ((bs1.(st) = bs2.(st)) /\ 
+            ((bs2.(BB_num) = jmp_dist1) /\ (test_true_jmp D bs1.(st)) \/ ((bs2.(BB_num) = jmp_dist2) /\ (test_false_jmp D bs1.(st)))));
+    Berr := ∅; (* Ignore err cases now *)
+    Binf := ∅;
+  |}.
+
+
+Definition jmp_sem (jmp_dist1: nat) (jmp_dist2: option nat)(D: option EDenote) :BDenote :=
+  match D with 
+  | None => ujmp_sem jmp_dist1 (* No expr *)
+  | Some D => match jmp_dist2 with
+              | None => ujmp_sem jmp_dist1
+              | Some jmp_dist2 => cjmp_sem jmp_dist1 jmp_dist2 D
+              end
+  end.
+
+Definition BAsgn_sem (x: var_name) (e:EDenote) : BDenote := {|
+  Bnrm := fun (bs1:BB_state) (bs2:BB_state) => 
+     exists i,
+     (e.(nrm) bs1.(st) i) /\  (bs2.(st) x = Vint i) /\ (forall y, x <> y -> bs1.(st) y = bs2.(st) y);
+  Berr := fun(bs1:BB_state) => bs1.(st) ∈ e.(err);
+  Binf := ∅;
+|}.
+
+
+Definition BJump_sem (jmp_dist1: nat) (jmp_dist2: option nat) (D: option EDenote) : BDenote := {|
+  Bnrm := fun bs1 bs2 => 
+    exists i,
+      bs1.(st) = i.(st) /\ (jmp_sem jmp_dist1 jmp_dist2 D).(Bnrm) i bs2;
+  Berr := ∅;
+  Binf := ∅;
+|}.
+
+(** Now we are certain that BB only contains BAsgn and BJump cmds *)
+(* The sementics for a list of BAsgn *)
+Print BB_cmd.
+
+
+Definition BAsgn_denote (BAsgn_cmd: BB_cmd) : BDenote :=   
+  let x := BAsgn_cmd.(X) in 
+  let e := BAsgn_cmd.(E) in
+ {|
+  Bnrm :=  fun (bs1: BB_state) (bs2: BB_state) => (BAsgn_sem x (eval_expr e)).(Bnrm) bs1 bs2 /\ (bs1.(BB_num) = bs2.(BB_num)); 
+  Berr := (BAsgn_sem x (eval_expr e)).(Berr);
+  Binf := ∅;
+|}.
+
+
+
+Fixpoint BAsgn_list_sem (BAsgn_list: list BB_cmd) : BDenote := 
+match BAsgn_list with 
+ | BAsgn_cmd :: tl =>
+   {|   
+      Bnrm := (BAsgn_denote BAsgn_cmd).(Bnrm) ∘ (BAsgn_list_sem tl).(Bnrm);
+      Berr := (BAsgn_denote BAsgn_cmd).(Berr) ∪ (BAsgn_denote BAsgn_cmd).(Bnrm) ∘ (BAsgn_list_sem tl).(Berr);
+      Binf := ∅;
+  |}
+  | _ =>
+  {|
+      Bnrm := Rels.id;
+      Berr := ∅;
+      Binf := ∅;
+  |}
+end.
+
+Definition eval_cond_expr (e: option expr): option EDenote :=
+  match e with
+  | Some (EBinop op e1 e2) =>
+      Some (binop_sem op (element_sem (e1)) (element_sem (e2)))
+  | Some (EUnop op e1) =>
+      Some (unop_sem op (element_sem (e1)))
+  | None => None
+  end.
+
+
+(* Combine list of BAsgn and the final BJump *)
+Definition BB_sem (BB: BasicBlock): BDenote := {| 
+  Bnrm := 
+    let jmp_dist1 := BB.(jump_info).(jump_dist_1) in
+    let jmp_dist2 := BB.(jump_info).(jump_dist_2) in
+    let jmp_cond := BB.(jump_info).(jump_condition) in
+    (BAsgn_list_sem BB.(cmd)).(Bnrm) ∘ (BJump_sem jmp_dist1 jmp_dist2 (eval_cond_expr jmp_cond)).(Bnrm); 
+  Berr := ∅;
+  Binf := ∅;
+|}.
+
+
+(* Combine the single_step_stem to form the denotation for BB_list_sem.
+   Not certain about its correctness  *)
+Fixpoint BB_list_sem (BBs: list BasicBlock): BDenote := {|
+  Bnrm := 
+    match BBs with 
+    | BB :: tl => (BB_sem BB).(Bnrm) ∘ (BB_list_sem tl).(Bnrm)
+    | _ => Rels.id
+    end;
+  Berr := ∅;
+  Binf := ∅;
+|}.
+
+
+(* Construct the denotation for the original cmds, should be in cmd_denotations.v 
+* For debugging convenience, I have put it here
+*)
+
+(* The definition follows similar approach as BB_gen for mutually recursive cases *)
+Section cmd_list_sem.
+
+Variable cmd_sem : cmd -> CDenote.
+
+Fixpoint cmd_list_sem (cmd_list: list cmd): CDenote := {|
+  nrm := 
+    match cmd_list with
+    | cmd :: tl => (cmd_sem cmd).(nrm) ∘ (cmd_list_sem tl).(nrm)
+    | _ => Rels.id
+    end;
+  err := ∅;
+  inf := ∅;
+|}.
+
+End cmd_list_sem.
+
+(* I have used while_sem from cmd_denotations.v, don't know if it is correct *)
+Fixpoint cmd_sem (cmd: cmd): CDenote := {|
+  nrm := 
+    match cmd with 
+    | CAsgn x e => (asgn_sem x (eval_expr e)).(nrm)
+    | CIf e c1 c2 => (if_sem (eval_expr e) (cmd_list_sem cmd_sem c1) (cmd_list_sem cmd_sem c2)).(nrm)
+    | CWhile pre e body => (while_sem (eval_expr e) (cmd_list_sem cmd_sem body) (cmd_list_sem cmd_sem pre)).(nrm)
+    end;
+  err := ∅;
+  inf := ∅;
+|}.
+
+Definition state_to_BBstate (s: state): BB_state :=
+  {| BB_num := 0; st := s |}.
+
+(* The following are the equivalence between BB_state and state *)
+
+
+(* The following are preparations for the final theorem *)
+
+
+Record BCequiv (B: BDenote) (C: CDenote) (startBB endBB: nat): Prop := {
+  nrm_cequiv: (fun s1 s2 => exists bs1 bs2, B.(Bnrm) bs1 bs2 /\ bs1.(st) = s1 /\ bs2.(st) = s2 /\ bs1.(BB_num) = startBB /\ bs2.(BB_num) = endBB) == C.(nrm);
+  err_cequiv: (fun s => exists bs, B.(Berr) bs /\ bs.(st) = s) == C.(err); 
+  inf_cequiv: (fun s => exists bs, B.(Binf) bs /\ bs.(st) = s) == C.(inf);
+}.
+
+(* 
+Notation "c1 '~=~' c2" := (cequiv c1 c2)
+  (at level 69, only printing, no associativity). *)
+
+
+Definition construct_BB_state (s: state) (BB_num: nat): BB_state := 
+  {| BB_num := BB_num; st := s |}.
+
+
+Check Rels_concat_id_l.
+
+Check Rels_concat_id_r.
+
+
+
+
+Ltac my_destruct H :=
+  match type of H with 
+  | exists _, _ => destruct H as [? H]; my_destruct H 
+  | _ /\ _ => let H1:= fresh "H" in 
+              destruct H as [H H1];my_destruct H; my_destruct H1
+  | _ => idtac 
+  end.
+
+
+
+Definition start_with_Asgn (cmds: list cmd) : Prop :=
+  match cmds with
+  | CAsgn _ _ :: _ => True
+  | _ => False
+  end.
+
+
+
+Definition Q(c: cmd): Prop :=
+  (* Q(Asgn)里面不能出现cmds, 或者说Q(c)里面你就要讲BBs等等变化前后有什么区别, 别去搞cmds，你们搞得那个反而把问题搞复杂了
+    嗯，当然你要证明的是语义的变化，所以你要说多出来的commands的语义，和那个c的语义一样 -- by cqx *)
+  forall (BBs: list BasicBlock) (BBnow: BasicBlock) (BBnum :nat), 
+    let res := cmd_BB_gen c BBs BBnow BBnum in
+    (*CAsgn*)
+    (exists BBnow' BBcmd,
+      res.(BBn) = BBnow' /\
+      BBnow'.(commands) = BBnow.(commands) ++ (BBcmd :: nil) /\
+      BCequiv (BAsgn_list_sem (BBcmd :: nil)) (cmd_sem c) BBnow'.(block_num) BBnow'.(block_num)) (*还在当下的BBnow里，BBnum则是下一个BB的编号，不能用*)
+    \/
+    (*CIf / CWhile*)
+    (exists BBs' BBnum', 
+      res.(BasicBlocks) =  BBs ++ (BBnow :: nil) ++ BBs' /\
+      res.(BBn).(block_num) = BBnum' /\
+      BCequiv (BB_list_sem BBs') (cmd_sem c) BBnum BBnum').
+
+
+(* c: the cmd we are currently facing
+  BBs: list of Basic Blocks which have been already generated
+  BB_now: the Basic Block we are currently at
+  BB_num: we should start assigning new basic blocks with BB_num 
+  
+  Record basic_block_gen_results : Type := {
+  BasicBlocks: list BasicBlock; (* already finished blocks*)
+  BBn: BasicBlock; (* current_block_num should be the block num of BB_now, I think *)
+  next_block_num: nat (* I think next block should start with the number*)
+}.*)
+
+Definition P(cmds: list cmd): Prop :=
+  forall (BBs: list BasicBlock) (BBnow: BasicBlock) (BBnum :nat),  exists BBs' BBnow' BBcmd c tl,
+    let res := list_cmd_BB_gen cmd_BB_gen cmds BBs BBnow BBnum in
+    let BBres := res.(BasicBlocks) ++ (res.(BBn) :: nil) in
+
+    (* Start with CAsgn*)
+    cmds = c :: tl /\ res.(BBn) = BBnow' /\ BBnow'.(commands) = BBnow.(commands) ++ (BBcmd :: nil) /\ 
+    BBres = BBs ++ (BBnow'::nil) ++ BBs' /\ BCequiv (BAsgn_list_sem (BBcmd :: nil)) (cmd_sem c) BBnow'.(block_num) BBnow'.(block_num) /\ 
+    BCequiv (BB_list_sem BBs') (cmd_list_sem cmd_sem cmds) BBnum res.(BBn).(block_num)
+    \/
+    (* Start with CIf or CWhile *)
+    BBres = BBs ++ (BBnow :: nil) ++ BBs' /\ BCequiv (BB_list_sem BBs') (cmd_list_sem cmd_sem cmds) BBnum res.(BBn).(block_num).
+
+
+
+Lemma Q_asgn:
+  forall (x: var_name) (e: expr),
+  Q (CAsgn x e).
+Proof.
+  intros. unfold Q. left.
+  exists {|
+    block_num := BBnow.(block_num);
+    commands := BBnow.(cmd) ++ {| X:= x; E:= e|} :: nil;
+    jump_info := BBnow.(jump_info);
+  |}.
+  exists {| X := x; E := e|}.
+  split.
+  + reflexivity.
+  + split. tauto. split.
+    - unfold BAsgn_list_sem. simpl.
+      sets_unfold. intros.
+      split; intros.
+      * destruct H as [? [? [? [? [? [? ?]]]]]].
+        destruct H as [? ?].
+        destruct H as [? ?].
+        destruct H as [[? ?] ?].
+        exists x3.
+        rewrite H0 in H.
+        rewrite <- H4 in H1.
+        rewrite H1 in H.
+        split. apply H. split. apply H.
+        destruct H as [? [? ?]].
+        intros.
+        specialize (H7 Y). apply H7 in H8.
+        rewrite H8. 
+        tauto.
+      * destruct H as [? [? [? ?]]].
+        exists {| st := a; BB_num := BBnow.(block_num) |}.
+        exists {| st := a0; BB_num := BBnow.(block_num) |}.
+        split.
+        ++ simpl.
+           exists {| st := a0; BB_num := BBnow.(block_num) |}.
+           split. split.
+           exists x0. simpl.
+           split. apply H. 
+           split. apply H0.
+           intros. specialize (H1 y). apply H1 in H2. rewrite H2. tauto.
+           simpl. tauto.
+           simpl. tauto.
+        ++ simpl. tauto.
+    - admit.
+    - admit. 
+Admitted.
+
+Lemma Q_if:
+  forall (e: expr) (c1 c2: list cmd),
+  P c1 -> P c2 -> Q (CIf e c1 c2).
+Proof.
+  intros.
+  unfold Q. intros. right.
+ 
+Admitted. 
+
+
+Lemma Q_while:
+  forall (pre: list cmd) (e: expr) (body: list cmd),
+  P pre -> P body -> Q (CWhile pre e body).
+Proof.
+Admitted.
+
+Lemma P_nil:
+  P nil.
+Proof.
+Admitted.
+
+
+
+Lemma P_cons:
+  forall (c: cmd) (cmds: list cmd),
+  Q c -> P cmds -> P (c :: cmds).
+Proof.
+Admitted.
+
+
+Theorem BB_sound:
+  forall (cmds: list cmd),
+  P cmds.
+Proof.
+  intros.
+  induction cmds.
+  - apply P_nil.
+  - apply P_cons.
+    + destruct a.
+      * apply Q_asgn.
+      * destruct cmds.
+Qed.
